src/Language/PlutusIR/Semantics/TypeSafety/SubstitutionPreservesTyping.v
@@ -1,0 +1,243 @@
+Require Import PlutusCert.Language.PlutusIR.
+Import NamedTerm.
+Require Import PlutusCert.Language.PlutusIR.Semantics.Static.
+Require Import PlutusCert.Language.PlutusIR.Semantics.Static.Implementations.Named.
+Require Import PlutusCert.Language.PlutusIR.Semantics.Static.Weakening.
+Require Import PlutusCert.Language.PlutusIR.Semantics.Dynamic.
+
+Require Import Coq.Strings.String.
+
+Axiom skip : forall P, P.
+
+Definition P_Term (t : Term) :=
+  forall ctx x U v T t',
+    extendT x U ctx |-+ t : T ->
+    emptyContext |-+ v : U ->
+    substitute x v t t' ->
+    ctx |-+ t' : T.
+#[export] Hint Unfold P_Term : core.
+
+Definition P_Binding (b : Binding) :=
+  forall ctx x U v b',
+    extendT x U ctx |-ok b ->
+    emptyContext |-+ v : U ->
+    substitute_binding x v b b' ->
+    ctx |-ok b' /\ binds b = binds b'.
+#[export] Hint Unfold P_Binding : core.
+
+Definition P_Bindings_NonRec (bs : list Binding) :=
+  forall ctx x U v bs',
+    extendT x U ctx |-oks_nr bs ->
+    emptyContext |-+ v : U ->
+    Util.ForallT P_Binding bs ->
+    substitute_bindings_nonrec x v bs bs' ->
+    ctx |-oks_nr bs'.
+
+Lemma e : forall bs, P_Bindings_NonRec bs.
+Proof.
+  induction bs.
+  - unfold P_Bindings_NonRec.
+    intros.
+    inversion H1. subst.
+    auto with typing.
+  - unfold P_Bindings_NonRec.
+    intros.
+    inversion H1.
+    + subst.
+      apply W_ConsB_NonRec.
+      * apply Util.ForallT_hd in X.
+        unfold P_Binding in X.
+        eapply X.
+        -- inversion H. subst.
+           apply H5.
+        -- apply H0.
+        -- assumption.
+      * apply Util.ForallT_hd in X.
+        unfold P_Binding in X.
+        inversion H. subst.
+        destruct (X _ _ _ _ _ H5 H0 H8).
+        rewrite <- H3.
+        apply skip.
+    + subst.
+      apply W_ConsB_NonRec.
+      * apply Util.ForallT_hd in X.
+        apply X with x U v.
+        -- inversion H. subst.
+           assumption.
+        -- assumption.
+        -- assumption.
+      * eapply IHbs.
+        -- inversion H. subst.
+           apply skip.
+        -- apply H0.
+        -- apply Util.ForallT_tl in X.
+           assumption.
+        -- apply H9.
+Qed.
+
+Lemma substitution_preserves_typing : forall t, P_Term t.
+Proof.
+  apply Term_rect' with (P := P_Term) (Q := P_Binding).
+  - intros. autounfold. intros.
+    inversion H2.
+    + subst.
+      eapply T_Let.
+      * reflexivity.
+      * eapply e.
+        -- inversion H0. subst.
+            eauto.
+        -- eauto.
+        -- eauto.
+        -- eauto.
+      * inversion H0. subst.
+        apply skip.
+    + subst.
+      inversion H0. subst.
+      eapply T_Let.
+      * reflexivity.
+      * eapply e.
+        -- inversion H0. subst.
+           eauto.
+        -- eauto.
+        -- eauto.
+        -- eauto.
+      * apply skip.
+    + apply skip.
+    + apply skip.
+  - intros. autounfold. intros.
+    inversion H1.
+    + subst.
+      inversion H.
+      subst.
+      inversion H4.
+      rewrite update_eq in H3.
+      inversion H3. subst. 
+      eapply weakening_empty; eauto.
+    + subst.
+      apply T_Var.
+      inversion H.
+      subst.
+      simpl in H4.
+      rewrite update_neq in H4; auto.
+  - (* TyAbs *) 
+    intros. autounfold. intros.
+    inversion H2. subst.
+    inversion H0. subst.
+    apply T_TyAbs.
+    rewrite extendT_extendK_permute in H8.
+    eapply H.
+    + eauto.
+    + eauto.
+    + eauto.
+  - (* LamAbs *)
+    intros. autounfold. intros.
+    inversion H0. subst.
+    inversion H2.
+    + subst.
+      apply T_LamAbs.
+      * rewrite extendT_shadow in H8.
+        assumption.
+      * apply skip.
+    + subst.
+      apply T_LamAbs.
+      * eapply H.
+        -- rewrite extendT_permute in H8; auto.
+           apply H8.
+        -- eassumption.
+        -- assumption.
+      * apply skip.
+  - (* Apply *)
+    intros. autounfold. intros.
+    inversion H1. subst.
+    inversion H3. subst.
+    eapply T_Apply.
+    + eapply H.
+      * eassumption.
+      * eassumption.
+      * assumption.
+    + eapply H0.
+      * eassumption.
+      * eassumption.
+      * assumption.
+  - (* Constant *)
+    intros. autounfold. intros.
+    inversion H. subst.
+    inversion H1. subst.
+    apply T_Constant.
+  - (* Builtin *) 
+    intros. autounfold. intros.
+    inversion H. subst.
+    inversion H1. subst.
+    apply T_Builtin.
+  - (* TyInst *)
+    intros. autounfold. intros.
+    inversion H0. subst.
+    inversion H2. subst.
+    eapply T_TyInst.
+    + eapply H.
+      * eassumption.
+      * eassumption.
+      * eassumption.
+    + apply skip.
+    + assumption.
+  - (* Error *)
+    intros. autounfold. intros.
+    inversion H. subst.
+    inversion H1. subst.
+    apply T_Error.
+    apply skip.
+  - (* IWrap *)
+    intros. autounfold. intros.
+    inversion H0. subst.
+    inversion H2. subst.
+    eapply T_IWrap.
+    + eassumption.
+    + eapply H.
+      * eassumption.
+      * eassumption.
+      * eassumption.
+    + apply skip.
+    + apply skip.
+  - (* Unwrap *)
+    intros. autounfold. intros.
+    inversion H0. subst.
+    inversion H2. subst.
+    eapply T_Unwrap.
+    + eapply H.
+      * eassumption.
+      * eassumption.
+      * assumption.
+    + apply skip.
+    + eassumption.
+
+  - (* TermBind *)
+    intros. autounfold. intros.
+    inversion H0. subst.
+    inversion H2. subst. 
+    split.
+    + apply W_Term.
+      * apply skip.
+      * eapply H.
+        -- eassumption.
+        -- eassumption.
+        -- assumption.
+    + reflexivity. 
+  - (* TypeBind *)
+    intros. autounfold. intros.
+    inversion H. subst.
+    inversion H1. subst.
+    split. 
+    + apply W_Type.
+      apply skip.
+    + reflexivity.
+  - (* DatatypeBind *)
+    intros. autounfold. intros.
+    inversion H. subst.
+    inversion H1. subst.
+    split.
+    + eapply W_Data.
+      * reflexivity.
+      * intros.
+        apply skip.
+    + reflexivity.
+Qed.
